progs/float.v
@@ -99,7 +99,7 @@ Definition composites : list composite_definition :=
    ((_x, tint) :: (_y, tfloat) :: (_z, tdouble) :: nil)
    noattr :: nil).
 
-Definition global_definitions :=
+Definition global_definitions : list (ident * globdef fundef type) :=
 ((___builtin_bswap,
    Gfun(External (EF_builtin "__builtin_bswap"
                    (mksignature (AST.Tint :: nil) (Some AST.Tint) cc_default))
