progs/int_or_ptr.v
@@ -161,7 +161,7 @@ Definition v_arena := {|
 
 Definition v_next := {|
   gvar_info := (tptr (Tstruct _tree noattr));
-  gvar_init := (Init_addrof _arena (Int.repr 0) :: nil);
+  gvar_init := (Init_addrof _arena (Ptrofs.repr 0) :: nil);
   gvar_readonly := false;
   gvar_volatile := false
 |}.
@@ -506,7 +506,7 @@ Definition composites : list composite_definition :=
     (_right, (talignas 2%N (tptr tvoid))) :: nil)
    noattr :: nil).
 
-Definition global_definitions :=
+Definition global_definitions : list (ident * globdef fundef type) :=
 ((___builtin_bswap,
    Gfun(External (EF_builtin "__builtin_bswap"
                    (mksignature (AST.Tint :: nil) (Some AST.Tint) cc_default))
