progs/nest3.v
@@ -271,7 +271,7 @@ Definition composites : list composite_definition :=
    ((_z1, (Tstruct _b noattr)) :: (_z2, (Tstruct _b noattr)) :: nil)
    noattr :: nil).
 
-Definition global_definitions :=
+Definition global_definitions : list (ident * globdef fundef type) :=
 ((___builtin_bswap,
    Gfun(External (EF_builtin "__builtin_bswap"
                    (mksignature (AST.Tint :: nil) (Some AST.Tint) cc_default))
