progs/ptr_compare.v
@@ -72,7 +72,7 @@ Definition f_f := {|
 Definition composites : list composite_definition :=
 nil.
 
-Definition global_definitions :=
+Definition global_definitions : list (ident * globdef fundef type) :=
 ((___builtin_bswap,
    Gfun(External (EF_builtin "__builtin_bswap"
                    (mksignature (AST.Tint :: nil) (Some AST.Tint) cc_default))
