Makefile
@@ -355,7 +355,16 @@ AES_FILES = \
 #  verif_hmac_drbg_update.v verif_hmac_drbg_reseed.v verif_hmac_drbg_generate.v
 
 
-C_FILES = reverse.c queue.c queue2.c sumarray.c sumarray2.c message.c object.c insertionsort.c float.c global.c nest3.c nest2.c nest3.c load_demo.c dotprod.c string.c field_loadstore.c ptr_compare.c merge.c append.c bst.c min.c switch.c funcptr.c store_demo.c floyd_tests.c int_or_ptr.c union.c
+# SINGLE_C_FILES are those that can be clightgen'd individually
+# NORMAL_C_FILES are those to be clightgen'd individually with -normalize flag
+# LINKED_C_FILES are those that need to be clightgen'd in a batch with others
+
+SINGLE_C_FILES = reverse.c revarray.c queue.c queue2.c message.c object.c insertionsort.c float.c global.c logical_compare.c nest2.c nest3.c ptr_compare.c load_demo.c store_demo.c dotprod.c string.c field_loadstore.c merge.c append.c bin_search.c bst.c bst_oo.c min.c switch.c funcptr.c floyd_tests.c incr.c
+
+NORMAL_C_FILES = sumarray.c sumarray2.c int_or_ptr.c union.c 
+
+LINKED_C_FILES = even.c odd.c
+C_FILES = $(SINGLE_C_FILES) $(NORMAL_C_FILES) $(LINKED_C_FILES)
 
 FILES = \
  $(MSL_FILES:%=msl/%) \
@@ -473,6 +482,8 @@ CGFLAGS =  -DCOMPCERT
 
 $(patsubst %.c,progs/%.vo,$(C_FILES)): compcert
 
+CVFILES = $(patsubst %.c,progs/%.v,$(C_FILES))
+
 cvfiles: $(CVFILES)
 
 dochtml:
@@ -487,60 +498,17 @@ clean_cvfiles:
 	rm $(CVFILES)
 
 ifdef CLIGHTGEN
+# SPECIAL-CASE RULES FOR LINKED_C_FILES:
 sha/sha.v sha/hmac.v hmacdrbg/hmac_drbg.v sha/hkdf.v: sha/sha.c sha/hmac.c hmacdrbg/hmac_drbg.c sha/hkdf.c
-	$(CLIGHTGEN) ${CGFLAGS} sha/sha.c sha/hmac.c hmacdrbg/hmac_drbg.c sha/hkdf.c
-# Is there a way to generate the next 5 rules automatically from C_FILES? 
-progs/revarray.v: progs/revarray.c
-	$(CLIGHTGEN) ${CGFLAGS} $<
-progs/reverse.v: progs/reverse.c
-	$(CLIGHTGEN) ${CGFLAGS} $<
-progs/queue.v: progs/queue.c
-	$(CLIGHTGEN) ${CGFLAGS} $<
-progs/queue2.v: progs/queue2.c
-	$(CLIGHTGEN) ${CGFLAGS} $<
-progs/sumarray.v: progs/sumarray.c
-	$(CLIGHTGEN) -normalize ${CGFLAGS} $<
-progs/sumarray2.v: progs/sumarray2.c
-	$(CLIGHTGEN) -normalize ${CGFLAGS} $<
-progs/message.v: progs/message.c
-	$(CLIGHTGEN) ${CGFLAGS} $<
-progs/object.v: progs/object.c
-	$(CLIGHTGEN) ${CGFLAGS} $<
-progs/insertionsort.v: progs/insertionsort.c
-	$(CLIGHTGEN) ${CGFLAGS} $<
-progs/float.v: progs/float.c
-	$(CLIGHTGEN) ${CGFLAGS} $<
-progs/global.v: progs/global.c
-	$(CLIGHTGEN) ${CGFLAGS} $<
-progs/logical_compare.v: progs/logical_compare.c
-	$(CLIGHTGEN) ${CGFLAGS} $<
-progs/nest2.v: progs/nest2.c
-	$(CLIGHTGEN) ${CGFLAGS} $<
-progs/nest3.v: progs/nest3.c
-	$(CLIGHTGEN) ${CGFLAGS} $<
-progs/ptr_compare.v: progs/ptr_compare.c
-	$(CLIGHTGEN) ${CGFLAGS} $<
-progs/dotprod.v: progs/dotprod.c
-	$(CLIGHTGEN) ${CGFLAGS} $<
-progs/string.v: progs/string.c
-	$(CLIGHTGEN) ${CGFLAGS} $<
+	$(CLIGHTGEN) ${CGFLAGS} $^
 progs/even.v: progs/even.c progs/odd.c
-	$(CLIGHTGEN) ${CGFLAGS} $<
+	$(CLIGHTGEN) ${CGFLAGS} $^
 progs/odd.v: progs/even.v
-progs/field_loadstore.v: progs/field_loadstore.c
-	$(CLIGHTGEN) ${CGFLAGS} $<
-progs/merge.v: progs/merge.c
-	$(CLIGHTGEN) ${CGFLAGS} $<
-progs/append.v: progs/append.c
-	$(CLIGHTGEN) ${CGFLAGS} $<
-progs/switch.v: progs/switch.c
-	$(CLIGHTGEN) ${CGFLAGS} $<
-progs/funcptr.v: progs/funcptr.c
-	$(CLIGHTGEN) ${CGFLAGS} $<
-progs/int_or_ptr.v: progs/int_or_ptr.c
-	$(CLIGHTGEN) ${CGFLAGS}  -normalize $<
-progs/union.v: progs/union.c
-	$(CLIGHTGEN) ${CGFLAGS}  -normalize $<
+# GENERAL RULES FOR SINGLE_C_FILES and NORMAL_C_FILES
+$(patsubst %.c,progs/%.v, $(SINGLE_C_FILES)): progs/%.v: progs/%.c
+	$(CLIGHTGEN) ${CGFLAGS} $^
+$(patsubst %.c,progs/%.v, $(NORMAL_C_FILES)): progs/%.v: progs/%.c
+	$(CLIGHTGEN) ${CGFLAGS} -normalize $^
 endif
 
 version.v:  VERSION $(MSL_FILES:%=msl/%) $(SEPCOMP_FILES:%=sepcomp/%) $(VERIC_FILES:%=veric/%) $(FLOYD_FILES:%=floyd/%)
